src/travorder/TravOrderConfig.v
@@ -17,211 +17,18 @@ Require Import AuxRel2.
 Require Import TraversalOrder.
 Require Import travorder.IordTraversal.
 Require Import AuxRel2.
-(* Require Import SimTravClosure. *)
-
+Require Import IordCoherency.
 
 Import ListNotations.
 
 Set Implicit Arguments.
-
-Definition iord_coherent (G: execution) (sc: relation actid) (tc: trav_label -> Prop) 
-  := dom_rel (iord G sc ;; <|tc|>) ⊆₁ tc.
-
-(* TODO: move to TraversalOrder.v *)
-Global Add Parametric Morphism : SB with signature
-       eq ==> same_relation ==> same_relation as SB_more.
-Proof using.
-  intros G r r' EQ.
-  unfold SB. rewrite EQ; eauto.
-Qed.
-
-(* TODO: move to ... *)
-Global Add Parametric Morphism : ar with signature
-       eq ==> same_relation ==> same_relation as ar_more.
-Proof using.
-  intros G r r' EQ.
-  now unfold ar; rewrite EQ.
-Qed.
-
-(* TODO: move to TraversalOrder.v *)
-Global Add Parametric Morphism : AR with signature
-       eq ==> same_relation ==> same_relation as AR_more.
-Proof using.
-  intros G r r' EQ.
-  unfold AR. now rewrite EQ.
-Qed.
-
-(* TODO: move to TraversalOrder.v *)
-Global Add Parametric Morphism : PROP with signature
-       eq ==> same_relation ==> same_relation as PROP_more.
-Proof using.
-  intros G r r' EQ.
-  unfold PROP. now rewrite EQ.
-Qed.
-
-(* TODO: move to TraversalOrder.v *)
-Global Add Parametric Morphism : iord with signature
-       eq ==> same_relation ==> same_relation as iord_more.
-Proof using.
-  intros G r r' EQ.
-  unfold iord.
-  apply restr_rel_more; eauto.
-  now rewrite EQ.
-Qed.
-
-Global Add Parametric Morphism : iord_coherent with signature
-       eq ==> same_relation ==> set_equiv ==> iff as iord_coherent_more.
-Proof using.
-  intros G sc sc' EQ s s' EQS.
-  unfold iord_coherent. 
-  split; intros HH.
-  { now rewrite <- EQS, <- EQ. }
-  now rewrite EQS, EQ.
-Qed.
-
-Record tls_coherent (G: execution) (tc: trav_label -> Prop): Prop :=
-  {
-    tls_coh_init: init_tls G ⊆₁ tc;
-    (* tls_coh_exec: tc \₁ event ↓₁ is_init ⊆₁ exec_tls G *)
-    tls_coh_exec: tc ⊆₁ init_tls G ∪₁ exec_tls G
-  }.
-
-Definition tls_coherent_alt (G: execution) (tc: trav_label -> Prop) :=
-  exists tc', tc' ⊆₁ exec_tls G /\ tc ≡₁ init_tls G ∪₁ tc'. 
-
-Lemma tls_coherent_defs_equiv (G: execution) (tc: trav_label -> Prop):
-  tls_coherent G tc <-> tls_coherent_alt G tc. 
-Proof using. 
-  split; intros COH. 
-  2: { red in COH. desc. split; rewrite ?COH0, ?COH; basic_solver. }
-  destruct COH. red. exists (tc \₁ init_tls G). split.
-  { rewrite tls_coh_exec0. basic_solver. }
-  split; [| basic_solver]. 
-  rewrite (set_split_complete (init_tls G) tc) at 1. basic_solver.
-Qed.
-    
-
-Section CoherentConfigs. 
-  Variable (G: execution) (sc: relation actid). 
-  Variable (tc: trav_label -> Prop). 
-
-  (* Hypothesis (FITS: fits_graph G tc).  *)
-  (* Hypothesis (COH: iord_coherent G sc tc). *)
-  Notation "'sb'" := (sb G).
-  Notation "'rmw'" := (rmw G).
-  Notation "'data'" := (data G).
-  Notation "'addr'" := (addr G).
-  Notation "'ctrl'" := (ctrl G).
-  Notation "'rf'" := (rf G).
-  Notation "'co'" := (co G).
-  Notation "'coe'" := (coe G).
-  Notation "'fr'" := (fr G).
-
-  Notation "'fwbob'" := (fwbob G).
-  Notation "'ppo'" := (ppo G).
-  Notation "'ar'" := (ar G sc).
-  Notation "'fre'" := (fre G).
-  Notation "'rfi'" := (rfi G).
-  Notation "'rfe'" := (rfe G).
-  Notation "'deps'" := (deps G).
-  Notation "'detour'" := (detour G).
-
-  Notation "'lab'" := (lab G).
-  Notation "'loc'" := (loc lab).
-  Notation "'val'" := (val lab).
-  Notation "'mod'" := (Events.mod lab).
-  Notation "'same_loc'" := (same_loc lab).
-  
-  Notation "'E'" := (acts_set G).
-  Notation "'R'" := (fun x => is_true (is_r lab x)).
-  Notation "'W'" := (fun x => is_true (is_w lab x)).
-  Notation "'F'" := (fun x => is_true (is_f lab x)).
-  Notation "'Sc'" := (fun x => is_true (is_sc lab x)).
-  Notation "'RW'" := (R ∪₁ W).
-  Notation "'FR'" := (F ∪₁ R).
-  Notation "'FW'" := (F ∪₁ W).
-  Notation "'R_ex'" := (fun a => is_true (R_ex lab a)).
-  Notation "'W_ex'" := (W_ex G).
-  Notation "'W_ex_acq'" := (W_ex ∩₁ (fun a => is_true (is_xacq lab a))).  
-  Notation "'Rel'" := (fun x => is_true (is_rel lab x)).
-
-  Implicit Types (WF : Wf G) (COMP : complete G)
-           (WFSC : wf_sc G sc) (CONS : imm_consistent G sc)
-           (SCPL: sc_per_loc G)
-           (TCOH: tls_coherent G tc)
-           (ICOH: iord_coherent G sc tc).
-  
-  Lemma tlsc_I_in_W WF TCOH:
-    tc ∩₁ (action ↓₁ eq ta_issue) ⊆₁ event ↓₁ W. 
-  Proof using .
-    apply tls_coherent_defs_equiv in TCOH as [tc' [INE TC']].
-    rewrite TC', set_inter_union_l. apply set_subset_union_l. split.
-    { etransitivity; [red; intro; apply proj1| ].
-      unfold init_tls. erewrite set_pair_alt, init_w; eauto. basic_solver. }
-    rewrite INE. unfold exec_tls. rewrite !set_pair_alt.
-    unfold action, event. unfolder. ins; desf; congruence.  
-  Qed.
-  
-  Lemma tlsc_P_in_W thread WF TCOH:
-    tc ∩₁ (action ↓₁ eq (ta_propagate thread)) ⊆₁ event ↓₁ W. 
-  Proof using. 
-    apply tls_coherent_defs_equiv in TCOH as [tc' [INE TC']].
-    rewrite TC', set_inter_union_l. apply set_subset_union_l. split.
-    { etransitivity; [red; intro; apply proj1| ].
-      unfold init_tls. erewrite set_pair_alt, init_w; eauto. basic_solver. }
-    rewrite INE. unfold exec_tls. rewrite !set_pair_alt.
-    unfold action, event. unfolder. ins; desf; congruence.  
-  Qed. 
-
-  Lemma exec_tls_ENI:
-    exec_tls G ⊆₁ event ↓₁ (E \₁ is_init).
-  Proof using. unfold exec_tls. rewrite !set_pair_alt. basic_solver. Qed.
-
-  Lemma init_tls_EI:
-    init_tls G ⊆₁ event ↓₁ (E ∩₁ is_init).
-  Proof using. unfold init_tls. rewrite !set_pair_alt. basic_solver. Qed.
-
-  Lemma tlsc_E WF TCOH:
-    tc ⊆₁ event ↓₁ E.
-  Proof using.
-    destruct TCOH. rewrite tls_coh_exec0, exec_tls_ENI, init_tls_EI. basic_solver.
-  Qed. 
-
-  Definition tlsI := tc ∩₁ (action ↓₁ eq ta_issue).
-  Definition tlsC := tc ∩₁ (action ↓₁ eq ta_cover).
-
-  
-  Lemma tlsc_w_covered_issued TCOH ICOH:
-    (* (* event ↑₁ (tc ∩₁ (action ↓₁ eq ta_cover)) ∩₁ W ⊆₁ event ↑₁ (tc ∩₁ (action ↓₁ eq ta_issue)). *) *)
-    (* ts_covered ∩₁ W ⊆₁ ts_issued. *)
-
-    (* tc ∩₁ (event ↓₁ W) ∩₁ (action ↓₁ eq ta_cover) ⊆₁ event ↓₁ (event ↑₁ (tc ∩₁ action ↓₁ eq ta_issue)). *)
-
-    tlsC ∩₁ (event ↓₁ W) ⊆₁ event ↓₁ (event ↑₁ tlsI).
-    (* (fun ae => mkTL ta_issue (event ae)) ↓₁ (tlsC ∩₁ (event ↓₁ W)) ⊆₁ tlsI. *)
-  Proof using.
-    destruct TCOH. unfold tlsC, tlsI.
-    unfolder. ins. desc. destruct x as [a e]. ins. subst.
-    
-    exists (mkTL ta_issue e). splits; eauto.
-    destruct (tls_coh_exec0 _ H) as [Il | EXl].
-    { apply tls_coh_init0. split; [basic_solver| ]. 
-      apply init_tls_EI in Il. auto. }
-    red in ICOH. apply ICOH.     
-    red. eexists. apply seq_eqv_r. split; eauto.
-    red. apply exec_tls_ENI in EXl. red. splits; try by vauto.
-    do 4 left. right. red. basic_solver 10. 
-  Qed.
-
-
-End CoherentConfigs. 
 
 
 
 Section TravOrderConfig.
   Context (G : execution) (sc : relation actid).
   Implicit Types (WF : Wf G) (COMP : complete G)
-           (WFSC : wf_sc G sc) (CONS : imm_consistent G sc)
+           (CONS : imm_consistent G sc)
            (MF : mem_fair G).
 
   Notation "'sb'" := (sb G).
@@ -470,17 +277,6 @@ Lemma eqv_rel_alt {A: Type} (S: A -> Prop):
   ⦗S⦘ ≡ S × S ∩ eq.
 Proof using. basic_solver. Qed.
 
-Lemma icoh_clos_refl tc (ICOH: iord_coherent G sc tc):
-  dom_rel ((iord G sc)^? ⨾ ⦗tc⦘) ⊆₁ tc. 
-Proof using.
-  rewrite crE, seq_union_l, seq_id_l, dom_union.
-  red in ICOH. rewrite ICOH. basic_solver.
-Qed.
-
-Lemma set_compl_set_mapC {A B: Type} (d: B -> Prop) (f: A -> B):
-  set_compl (f ↓₁ d) ≡₁  (f ↓₁ set_compl d).
-Proof using. basic_solver. Qed. 
-
 Lemma doma_alt {A: Type} (r: relation A) (d: A -> Prop):
   doma r d <-> dom_rel r ⊆₁ d. 
 Proof using. unfolder. split; ins; basic_solver. Qed. 
@@ -499,7 +295,7 @@ Proof using.
   rewrite dom_union. apply set_subset_union_l. split.
   { rewrite wf_sbE. rewrite <- map_rel_seq_ext; [| by apply event_sur].
     rewrite <- !seqA. do 3 rewrite dom_seq. 
-    destruct TCOH. rewrite <- tls_coh_init0. unfold init_tls.
+    destruct TCOH. rewrite <- tls_coh_init. unfold init_tls.
     rewrite set_pair_alt. unfolder. ins. desc. splits; vauto. }
 
   red in ICOH. rewrite <- ICOH at 2. apply dom_rel_mori.
@@ -512,32 +308,7 @@ Proof using.
   rewrite wf_sbE, no_sb_to_init at 1. rewrite restr_relE. basic_solver. 
 Qed. 
 
-
-(* Lemma clos_trans_restr_sur {A B: Type} (r: relation B) (d: A -> Prop) (f: A -> B) *)
-(*       (SUR_D: forall b, exists a, f a = b /\ d a): *)
-(*   (* f ↓₁ r^* ≡ (f ↓₁ r)^*.  *) *)
-(*   f ↓ r^* ≡ (f ↓ r)^*. *)
-(* Proof using.  *)
-(*   split. *)
-(*   2: { rewrite rtEE. apply inclusion_bunion_l. ins. induction x. *)
-(*        { simpl. basic_solver. } *)
-(*        rewrite pow_S_end, IHx. rewrite map_rel_seq, rt_unit. reflexivity. } *)
-(*   rewrite rtEE. apply inclusion_bunion_l. ins. induction x. *)
-(*   { unfolder. ins. red in H0. desc.  *)
-
-(* map_rel *)
-(* Lemma map_rel_dom_exact {A B: Type} (f: A -> B) (r: relation B) (d: A -> Prop) *)
-(*       (SUR_D: forall b, exists a, f a = b /\ d a): *)
-(*   f ↓ r ≡ restr_rel d (f ↓ r).  *)
-(* Proof using.  *)
-(*   split; [| basic_solver 10].  *)
-(*   unfolder. ins.  *)
-  
-
-(* Lemma map_rel_dom_exact {A B: Type} (f: A -> B) (r: relation B): *)
-(*   @set_full A ≡₁ f ↓₁ (@set_full B). *)
-(* Proof using. basic_solver. Qed. *)
-  
+(* TODO: move to lib *)  
 Lemma map_rel_seq_insert_exact {A B: Type} (r1 r2: relation B)
       (f: A -> B) (d: A -> Prop)
       (SUR_D: forall b, exists a, f a = b /\ d a):
@@ -548,30 +319,19 @@ Proof using.
 Qed. 
 
 
-(* Lemma ar_rf_ppo_loc_ct_coverable_issuable_in_I  : *)
-    (* dom_rel (⦗W⦘ ⨾ (ar ∪ rf ⨾ ppo ∩ same_loc)⁺ ⨾ ⦗coverable T ∪₁ issuable T⦘) ⊆₁ issued T. *)
-(* Lemma ar_rf_ppo_loc_ct_tls_cov_tls_iss tc: *)
-(*   dom_rel (event ↓ (⦗W⦘ ⨾ (ar ∪ rf ⨾ ppo ∩ same_loc)⁺) ⨾ ⦗tc ∩₁ action ↓₁ eq ta_cover⦘) ⊆₁ tc ∩₁ action ↓₁ eq ta_issue. *)
-(* Proof using. *)
-(*   rewrite map_rel_seq_insert_exact with (d := action ↓₁ eq ta_issue). *)
-(*   2: { ins. exists (mkTL ta_issue b). vauto. } *)
-(*   intros [a1 e1] [[a2 e2] REL%seq_eqv_r]. desc. *)
-(*   destruct REL0 as [TC2 [=<-]]. *)
-(*   red in REL. apply seq_eqv_l in REL as [We1 REL_CT]. ins.  *)
-
+(* TODO: move to lib *)  
 Lemma rel_map_bunionC {A B C: Type} (f: A -> B)
       (cdom: C -> Prop) (ss: C -> relation B):
   f ↓ (⋃ c ∈ cdom, ss c) ≡ (⋃ c ∈ cdom, f ↓ (ss c)).
 Proof using. basic_solver. Qed. 
 
+(* TODO: move to lib *)  
 Lemma dom_rel_bunion {B C: Type}
       (cdom: C -> Prop) (ss: C -> relation B):
   dom_rel (⋃ c ∈ cdom, ss c) ≡₁ (⋃₁ c ∈ cdom, dom_rel (ss c)).
 Proof using. basic_solver. Qed.
 
-(* Lemma dom_rel_restr_relC {A: Type} (r: relation A) (d: A -> Prop): *)
-(*   dom_rel (restr_rel d r) ≡ restr_rel d (d *)
-
+(* TODO: move to lib *)  
 Lemma restr_rel_seq_same {A: Type} (r1 r2: relation A) (d: A -> Prop)
       (DOMB1: domb (⦗d⦘ ⨾ r1) d):
   restr_rel d (r1 ⨾ r2) ≡ restr_rel d r1 ⨾ restr_rel d r2. 
@@ -581,105 +341,7 @@ Proof using.
   eexists. splits; eauto.
 Qed. 
 
-Definition iord_simpl : relation trav_label :=
-  SB G sc ∪ RF G ∪ FWBOB G ∪ AR G sc ∪ IPROP G ∪ PROP G sc.
-
-Definition E_ENI := E × (E \₁ is_init).
-
-Lemma sb_E_ENI: sb ⊆ E_ENI. 
-Proof using. rewrite wf_sbE, no_sb_to_init. basic_solver. Qed. 
-
-Lemma co_E_ENI WF (SCPL: sc_per_loc G): co ⊆ E_ENI. 
-Proof using. rewrite wf_coE, no_co_to_init; auto. basic_solver. Qed. 
-
-Lemma rf_E_ENI WF : rf ⊆ E_ENI. 
-Proof using. rewrite wf_rfE, no_rf_to_init; auto. basic_solver. Qed. 
-
-Lemma fr_E_ENI WF (SCPL: sc_per_loc G) : fr ⊆ E_ENI. 
-Proof using. rewrite wf_frE, no_fr_to_init; auto. basic_solver. Qed. 
-
-Lemma no_ar_to_init_alt CONS WF:
-  ar ≡ ar ⨾ ⦗set_compl is_init⦘. 
-Proof using.
-  forward eapply no_ar_to_init; eauto. basic_solver 10.
-  Unshelve. all: eauto.
-Qed. 
-
-Lemma ar_E_ENI WF WFSC CONS : ar ⊆ E_ENI. 
-Proof using. rewrite wf_arE, no_ar_to_init_alt; auto. basic_solver. Qed.
-
-Lemma sc_E_ENI WF WFSC: sc ⊆ E_ENI. 
-Proof using. rewrite wf_scE, (@no_sc_to_init _ WF _ WFSC); eauto. basic_solver. Qed.
-
-Lemma E_ENI_trans: transitive E_ENI.
-Proof using. unfold E_ENI. basic_solver. Qed.
-
-Lemma iord_simpl_E_ENI WF WFSC CONS:
-  iord_simpl ⊆ event ↓ E_ENI^?.
-Proof using. 
-  unfold iord_simpl. unfold SB, RF, FWBOB, AR, IPROP, PROP.
-  rewrite ppo_in_sb, fwbob_in_sb; auto. rewrite inclusion_inter_l1 with (r := sb).
-  rewrite ?sb_E_ENI, ?rf_E_ENI, ?co_E_ENI, ?fr_E_ENI, ?ar_E_ENI, ?sc_E_ENI; auto.
-  2: { cdes CONS. by apply imm_s_hb.coherence_sc_per_loc. }
-  rewrite <- !seqA. 
-  repeat (rewrite ?(@rt_of_trans _ E_ENI), ?(@rewrite_trans _ E_ENI),
-           ?unionK, ?(@rewrite_trans _ E_ENI),
-           ?(@rewrite_trans_seq_cr_cr _ E_ENI), ?(@ct_of_trans _ E_ENI)
-         ); auto using E_ENI_trans.
-  repeat rewrite inclusion_seq_eqv_l, inclusion_seq_eqv_r. basic_solver 10.
-Qed.
-
-(* Lemma iord_simpl_E_ENI_tc WF WFSC CONS tc: *)
-(*   iord_simpl ⨾ ⦗tc⦘ ⊆ event ↓ E_ENI ∪ ⦗tc⦘.  *)
-(* Proof using. *)
-(*   rewrite iord_simpl_E_ENI; auto. rewrite crE, map_rel_union, seq_union_l. *)
-(*   basic_solver 10.  *)
-
-Lemma iord_simpl_tc_doma WF WFSC CONS tc (TCOH: tls_coherent G tc):
-  doma (iord_simpl ⨾ ⦗tc⦘) (event ↓₁ E).
-Proof using.
-  rewrite iord_simpl_E_ENI; auto. rewrite crE, map_rel_union, seq_union_l.
-  apply union_doma.
-  { rewrite tlsc_E; eauto. unfolder. ins. desc. congruence. }
-  unfold E_ENI. basic_solver.
-Qed. 
   
-
-Lemma iord_coh_simpl WF WFSC CONS tc
-      (TCOH: tls_coherent G tc) (ICOH: iord_coherent G sc tc):
-  dom_rel (iord_simpl ⨾ ⦗tc⦘) ⊆₁ tc. 
-Proof using.
-  rewrite set_split_complete with (s' := dom_rel _) (s := event ↓₁ is_init).
-  forward eapply iord_simpl_tc_doma as IS_DOM%doma_rewrite; eauto.
-
-  apply set_subset_union_l. split.
-  { rewrite IS_DOM.     
-    destruct TCOH. rewrite <- tls_coh_init0 at 2. unfold init_tls.
-    rewrite set_pair_alt, set_map_inter.
-    rewrite <- set_interA. apply set_subset_inter; [| reflexivity].  
-    rewrite dom_eqv1, set_interC. apply set_subset_inter; [| reflexivity].
-    unfold iord_simpl. unfold SB, RF, FWBOB, AR, IPROP, PROP.
-    basic_solver 10. }
-  
-  rewrite set_interC, <- dom_eqv1.
-  red in ICOH. rewrite <- ICOH at 2. apply dom_rel_mori.
-  unfold iord. fold iord_simpl.
-  rewrite restr_relE. rewrite !seqA, seq_eqvC. 
-  rewrite set_minusE, set_map_inter, id_inter.
-  rewrite !seqA, seq_eqvC.
-  rewrite <- seqA with (r3 := ⦗_⦘ ⨾ ⦗_⦘). rewrite <- seqA with (r2 := _ ⨾ ⦗tc⦘).
-  rewrite set_compl_set_mapC.
-  etransitivity.
-  2: { apply seq_mori; [reflexivity| ].
-       rewrite <- id_inter. apply domb_rewrite.
-       rewrite iord_simpl_E_ENI; auto.
-       rewrite crE, map_rel_union. repeat case_union _ _. apply union_domb.
-       { rewrite (@tlsc_E G tc) at 1; eauto.
-         unfolder. ins. desc. split; congruence. }
-       unfold E_ENI. basic_solver. }
-  apply doma_rewrite. rewrite IS_DOM. basic_solver.
-Qed. 
-       
 Lemma iord_coherent_AR_ext_cover WF CONS tc
       (TCOH: tls_coherent G tc) (ICOH: iord_coherent G sc tc):
   dom_rel (((⦗action ↓₁ eq ta_issue⦘ ⨾ event ↓ (⦗W⦘ ⨾
@@ -708,7 +370,7 @@ Proof using.
   2: { ins. exists (mkTL ta_issue b). vauto. }
   rewrite map_rel_seq_insert_exact with (d := action ↓₁ eq ta_cover) at 1.
   2: { ins. exists (mkTL ta_cover b). vauto. }
-  apply iord_coh_simpl in ICOH; auto; [| by apply CONS]. 
+  apply iord_coh_implies_iord_simpl_coh in ICOH; auto. 
   repeat case_union _ _. rewrite dom_union. apply set_subset_union_l. split.
 
   { erewrite dom_rel_mori.
@@ -748,28 +410,12 @@ Proof using.
   etransitivity; [| by apply ICOH]. apply dom_rel_mori. hahn_frame.
   transitivity (AR G sc); [| unfold iord_simpl; basic_solver 10].
   unfold AR. basic_solver 10.
-Qed.   
-
-Lemma iord_simpl_clos_implies_iord_clos WF WFSC (tc: trav_label -> Prop)
-      (SIMPL_CLOS: dom_rel (iord_simpl ⨾ ⦗tc⦘) ⊆₁ tc):
-  iord_coherent G sc tc. 
-Proof using. 
-  red. erewrite dom_rel_mori; [by apply SIMPL_CLOS| ].
-  unfold iord, iord_simpl. basic_solver 10.
 Qed.
 
-Lemma iord_simpl_clos_refl WF WFSC CONS tc
-      (TCOH: tls_coherent G tc) (ICOH: iord_coherent G sc tc):
-  dom_rel ((iord_simpl)^? ⨾ ⦗tc⦘) ⊆₁ tc. 
-Proof using.
-  rewrite crE, seq_union_l, seq_id_l, dom_union.
-  red in ICOH. rewrite iord_coh_simpl; auto. basic_solver.
-Qed.
-
-Lemma sim_clos_iord_simpl_rmw_clos WF WFSC CONS (tc: trav_label -> Prop)
+Lemma sim_clos_iord_simpl_rmw_clos WF CONS (tc: trav_label -> Prop)
       (TCOH: tls_coherent G tc) (ICOH: iord_coherent G sc tc)
       :
-  dom_rel (iord_simpl ⨾ ⦗rmw_clos tc⦘) ⊆₁ tc ∪₁ rmw_clos tc ∪₁ rel_clos tc.
+  dom_rel (iord_simpl G sc ⨾ ⦗rmw_clos tc⦘) ⊆₁ tc ∪₁ rmw_clos tc ∪₁ rel_clos tc.
 Proof using.
   unfold iord_simpl. repeat case_union _ _. rewrite !dom_union.
   unfold rmw_clos. rewrite !set_pair_alt. 
@@ -786,7 +432,7 @@ Proof using.
     { apply dom_rel_mori.
       do 2 (apply seq_mori; [reflexivity| ]).
       apply union_mori; [reflexivity| ]. Unshelve. 2: exact (fun _ _ => False).
-      rewrite wf_scD, wf_rmwD; eauto. unfold event, action. type_solver 10. }
+      cdes CONS. rewrite wf_scD, wf_rmwD; eauto. unfold event, action. type_solver. }
     rewrite union_false_r. rewrite <- !id_inter.
     rewrite <- !set_interA.
     rewrite set_inter_absorb_r with (s' := _ ↓₁ (_ ∪₁ _)); [| basic_solver].
@@ -808,7 +454,8 @@ Proof using.
     rewrite rtE, map_rel_union. repeat case_union _ _. rewrite dom_union.
     apply set_subset_union_l. split.
     { iord_dom_solver. }
-    apply iord_coh_simpl in ICOH; auto. rewrite <- ICOH at 2. apply dom_rel_mori.
+    apply iord_coh_implies_iord_simpl_coh in ICOH; auto. rewrite <- ICOH at 2. 
+    apply dom_rel_mori.
     rewrite set_interC, id_inter.
     unfold iord_simpl, SB. basic_solver 10. }
   { unfold RF. rewrite crE, seq_union_r, map_rel_union.
@@ -826,7 +473,10 @@ Proof using.
     rewrite dom_rel_eqv_codom_rel.
     rewrite transp_seq, transp_eqv_rel, <- map_rel_transp.
     
-    etransitivity; [| apply iord_simpl_clos_refl; auto]. apply dom_rel_mori.
+    etransitivity; [| apply iord_simpl_coh_clos_refl].
+    2: { eapply iord_coh_implies_iord_simpl_coh; eauto. } 
+
+    apply dom_rel_mori.
     unfold iord_simpl. 
     repeat rewrite unionA. etransitivity.
     2: { apply seq_mori; [| reflexivity]. apply clos_refl_mori.
@@ -846,7 +496,7 @@ Proof using.
   rewrite ct_end, !seqA. unfold "ar" at 2.
   repeat rewrite seq_union_l with (r := ⦗W⦘).
   arewrite (sc ⨾ ⦗W⦘ ∪ rfe ⨾ ⦗W⦘ ⊆ ∅₂); [| rewrite union_false_l].
-  { rewrite (wf_scD WFSC), wf_rfeD; eauto. type_solver. }
+  { cdes CONS. rewrite (wf_scD Wf_sc), wf_rfeD; eauto. type_solver. }
   
   rewrite ar_int_in_sb; auto. arewrite (ppo ∩ same_loc ⊆ sb) at 2.
   { rewrite ppo_in_sb; basic_solver. }
@@ -889,6 +539,7 @@ Proof using.
   basic_solver 10.
 Qed.
 
+(* TODO: move to lib *)
 Lemma set_collect_map_ext [A B : Type] [f : A -> B] [d : B -> Prop]
       (SUR: forall b, exists a, f a = b):
   f ↑₁ (f ↓₁ d) ≡₁ d. 
@@ -898,30 +549,6 @@ Proof.
   specialize (SUR x) as [a Fa]. exists a. split; congruence. 
 Qed.
  
-(* Lemma set_map_collect_ext [A B : Type] (f : A -> B) (s : A -> Prop) *)
-(*       (SUR: forall b, exists a, f a = b): *)
-(*   s ≡₁ f ↓₁ (f ↑₁ s). *)
-(* Proof. *)
-(*   split; [apply set_map_collect| ]. *)
-(*   unfolder. ins. desc. *)
-
-(* Lemma dom_rel_set_map_collect_helper [A B : Type] (f1 f2: A -> B) (s : A -> Prop) (r: relation A) *)
-(*       (* (SUR: forall b, exists a, f a = b) *) *)
-(*       (* (SUR_D: forall b, exists a, f a = b /\ d a) *) *)
-(*   : *)
-(*   dom_rel ((f1 ↓ r) ⨾ ⦗f2 ↓₁ (f2 ↑₁ s)⦘) ≡₁ dom_rel (f1 ↓ r ⨾ ⦗s⦘). *)
-(* Proof. *)
-
-(* Lemma dom_rel_set_map_collect_helper [A B : Type] (f: A -> B) (s : A -> Prop) (r: relation A) *)
-(*       (* (SUR: forall b, exists a, f a = b) *) *)
-(*       (* (SUR_D: forall b, exists a, f a = b /\ d a) *) *)
-(*   : *)
-(*   dom_rel (r ⨾ ⦗f ↓₁ (f ↑₁ s)⦘) ≡₁ dom_rel (r ⨾ ⦗s⦘). *)
-(* Proof. *)
-(*   split. *)
-(*   2: { basic_solver 10. } *)
-(*   unfolder. ins. desc.  *)
-
 (* TODO: rename or adapt iord_dom_solver, since it doesn't always solve the goal *)
 Local Ltac iord_dom_unfolder :=
   unfold SB, RF, FWBOB, AR, PROP, IPROP;
@@ -936,9 +563,9 @@ Local Ltac iord_dom_unfolder :=
 Lemma sim_clos_iord_simpl_rel_clos WF CONS (tc: trav_label -> Prop)
       (TCOH: tls_coherent G tc) (ICOH: iord_coherent G sc tc)
       :
-  dom_rel (iord_simpl ⨾ ⦗rel_clos tc⦘) ⊆₁ tc ∪₁ rmw_clos tc ∪₁ rel_clos tc.
+  dom_rel (iord_simpl G sc ⨾ ⦗rel_clos tc⦘) ⊆₁ tc ∪₁ rmw_clos tc ∪₁ rel_clos tc.
 Proof using.  
-  pose proof ICOH as ICOH'. apply iord_coh_simpl in ICOH; auto; [| apply CONS]. 
+  pose proof ICOH as ICOH'. apply iord_coh_implies_iord_simpl_coh in ICOH; auto.
   unfold rel_clos at 1. rewrite !set_pair_alt. unfold iord_simpl. fold action event.
   repeat (case_union _ _; rewrite dom_union; apply set_subset_union_l; split).
   all: try by iord_dom_solver. 
@@ -983,16 +610,17 @@ Proof using.
     unfolder in d4. desc. ins; vauto. } 
 Qed. 
 
-Lemma sim_clos_iord_coherent WF WFSC CONS (tc: trav_label -> Prop)
+Lemma sim_clos_iord_coherent WF CONS (tc: trav_label -> Prop)
       (TCOH: tls_coherent G tc) (ICOH: iord_coherent G sc tc)
       :
       iord_coherent G sc (sim_clos tc). 
 Proof using.
-  apply iord_simpl_clos_implies_iord_clos; auto. 
+  apply iord_simpl_coh_implies_iord_coh; auto. 
   unfold sim_clos, iord_coherent.
-  rewrite !id_union, !seq_union_r, !dom_union.
+  red. rewrite !id_union, !seq_union_r, !dom_union.
   do 2 (try (apply set_subset_union_l; split)). 
-  { rewrite iord_coh_simpl; auto. basic_solver. }
+  { apply iord_coh_implies_iord_simpl_coh in ICOH; auto.
+    rewrite ICOH. basic_solver. }
   { apply sim_clos_iord_simpl_rmw_clos; auto. }
   apply sim_clos_iord_simpl_rel_clos; auto.
 Qed.
@@ -1019,22 +647,22 @@ Proof.
   eintros INIT%init_pln; eauto. mode_solver. 
 Qed. 
 
-  Global Add Parametric Morphism : sim_clos with signature
-      set_equiv ==> set_equiv as sim_clos_more.
-  Proof using.
-    unfold sim_clos. ins. unfold rmw_clos, rel_clos, tl_issued, tl_covered.
-    rewrite !set_pair_alt. rewrite H. basic_solver.
-  Qed.
+Global Add Parametric Morphism : sim_clos with signature
+       set_equiv ==> set_equiv as sim_clos_more.
+Proof using.
+  unfold sim_clos. ins. unfold rmw_clos, rel_clos, tl_issued, tl_covered.
+  rewrite !set_pair_alt. rewrite H. basic_solver.
+Qed.
 
-  Global Add Parametric Morphism : sim_clos_step with signature
-         set_equiv ==> set_equiv ==> iff as sim_clos_step_more.
-  Proof using. ins. apply set_extensionality in H, H0. by subst. Qed.
+Global Add Parametric Morphism : sim_clos_step with signature
+       set_equiv ==> set_equiv ==> iff as sim_clos_step_more.
+Proof using. ins. apply set_extensionality in H, H0. by subst. Qed.
 
-  Global Add Parametric Morphism
-         {A: Type} (r: relation (A -> Prop)):
-    r with signature
-         @set_equiv A ==> @set_equiv A ==> iff as set_equiv_rel_more. 
-  Proof using. ins. apply set_extensionality in H, H0. by subst. Qed.
+Global Add Parametric Morphism
+       {A: Type} (r: relation (A -> Prop)):
+  r with signature
+       @set_equiv A ==> @set_equiv A ==> iff as set_equiv_rel_more. 
+Proof using. ins. apply set_extensionality in H, H0. by subst. Qed.
 
 Section IssueClosure.
   Variable (tc: trav_label -> Prop). 
@@ -1048,15 +676,10 @@ Section IssueClosure.
   Hypothesis (ICOH': iord_coherent G sc tc').
   Hypothesis (TCOH: tls_coherent G tc). 
   Hypothesis (TCOH': tls_coherent G tc'). 
-  (* Hypothesis (TRAV_STEP : itrav_step G sc e tc tc').  *)
   Hypothesis (NISS: ~ tc lbl).
-  (* Hypothesis (ISS: issuable G sc tc e). *)
 
   Hypothesis (WF : Wf G)
-             (* (COMP : complete G) *)
-           (* (WFSC : wf_sc G sc) *)
-             (CONS : imm_consistent G sc)
-           (* (SCPL: sc_per_loc G) *). 
+             (CONS : imm_consistent G sc).
   
   Lemma ICOHs: iord_coherent G sc stc.
   Proof using WF TCOH ICOH CONS.
@@ -1075,7 +698,7 @@ Section IssueClosure.
     subst stc'. apply sim_clos_tls_coherent; auto; apply CONS.
   Qed. 
 
-  (* TODO: move upper*)
+  (* TODO: move to lib? *)
   Lemma set_subset_inter_exact {A: Type} (s s': A -> Prop):
     s ⊆₁ s' <-> s ⊆₁ s ∩₁ s'. 
   Proof using.
@@ -1084,19 +707,18 @@ Section IssueClosure.
   Qed.  
 
   Lemma iord_coh_intermediate
-        (* (LBL_NEW : set_compl stc (ta_issue, e)) *)
-        (* (RELw: is_rel lab e) *)
-        (STC': stc' ≡₁ stc ∪₁ eq (mkTL ta_issue w) ∪₁ eq (mkTL ta_cover w))
-    :
+        (STC': stc' ≡₁ stc ∪₁ eq (mkTL ta_issue w) ∪₁ eq (mkTL ta_cover w)):
     iord_coherent G sc (stc ∪₁ eq (mkTL ta_issue w)).
   Proof using WF TCOH' TCOH NISS ICOH' ICOH CONS.
-    assert (wf_sc G sc) as WFSC by apply CONS.
-    apply iord_simpl_clos_implies_iord_clos; auto.
+    (* assert (wf_sc G sc) as WFSC by apply CONS. *)
+    apply iord_simpl_coh_implies_iord_coh; auto.
 
-    rewrite id_union, seq_union_r, dom_union. apply set_subset_union_l. split.
-    { rewrite iord_coh_simpl; auto using ICOHs, TCOHs. basic_solver. }
+    red. rewrite id_union, seq_union_r, dom_union.
+    apply set_subset_union_l. split.
+    { rewrite iord_coh_implies_iord_simpl_coh; auto using ICOHs, TCOHs. 
+      basic_solver. }
 
-    pose proof ICOHs' as ICOHs'%iord_coh_simpl; auto using TCOHs'.
+    pose proof ICOHs' as ICOHs'%iord_coh_implies_iord_simpl_coh; auto using TCOHs'.
     rewrite STC' in ICOHs'.
     rewrite <- set_subset_union_r1, <- set_subset_union_r2 in ICOHs' at 1.
     rewrite set_subset_inter_exact in ICOHs'. rewrite set_subset_inter_exact.
@@ -1114,12 +736,12 @@ Section IssueClosure.
   Lemma trav_step_closures_isim_issue:
     sim_clos_step＊ stc stc'.
   Proof using WF TCOH' TCOH NISS ICOH' ICOH CONS.
-    assert (wf_sc G sc) as WFSC by apply CONS. 
     assert (W w) as Ww.
     { replace w with (event lbl); auto. eapply (@tlsc_I_in_W _ tc'); eauto. 
       subst tc'. basic_solver. }
     assert (~ tc (mkTL ta_cover w)) as NCw.
-    { intros Cw. forward eapply (@tlsc_w_covered_issued _ _ tc) as WCI; eauto.
+    { intros Cw.
+      forward eapply (@tlsc_w_covered_issued tc) as WCI; eauto.
       destruct NISS. specialize (WCI (mkTL ta_cover w)). specialize_full WCI.
       { basic_solver. }
       unfolder in WCI. desc. subst lbl. destruct y. simpl in *. subst.
@@ -1197,7 +819,7 @@ Qed.
   
 End IssueClosure.
             
-Lemma iord_step_implies_sim_clos_step WF WFSC CONS:
+Lemma iord_step_implies_sim_clos_step WF CONS:
   iord_step ⊆ sim_clos ↓ sim_clos_step^*.
 Proof using.
   unfolder; intros tc tc' STEP.
@@ -1207,7 +829,7 @@ Proof using.
   apply seq_eqv_l in AA. destruct AA as [COMPL AA].
   rewrite AA in *. clear dependent tc'.
 
-  assert (tls_coherent G tc) as TCOH.
+  assert (tls_coherent G tc /\ tls_coherent G (tc ∪₁ eq (a, e))) as [TCOH TCOH'].
   { admit. }
   assert (iord_coherent G sc (sim_clos tc)) as SIMCOH.
   { apply sim_clos_iord_coherent; auto. }
