src/travorder/IordCoherency.v
@@ -1,0 +1,225 @@
+Require Import Classical Peano_dec Setoid PeanoNat.
+From hahn Require Import Hahn.
+Require Import Lia.
+
+Require Import Events.
+Require Import Execution.
+Require Import Execution_eco.
+Require Import imm_bob.
+Require Import imm_s.
+Require Import imm_s_ppo.
+Require Import imm_s_rfppo.
+Require Import AuxDef.
+Require Import SetSize.
+Require Import FairExecution.
+Require Import ImmFair.
+Require Import AuxRel2.
+Require Import TraversalOrder.
+Require Import travorder.IordTraversal.
+Require Import AuxRel2.
+
+
+Definition iord_coherent G sc tc :=
+  dom_rel (iord G sc ⨾ ⦗tc⦘) ⊆₁ tc.
+
+Definition iord_simpl G sc : relation trav_label :=
+  SB G sc ∪ RF G ∪ FWBOB G ∪ AR G sc ∪ IPROP G ∪ PROP G sc.
+
+Definition iord_simpl_coherent G sc tc :=
+  dom_rel (iord_simpl G sc ⨾ ⦗tc⦘) ⊆₁ tc.
+
+Global Add Parametric Morphism : iord_coherent with signature
+       eq ==> same_relation ==> set_equiv ==> iff as iord_coherent_more.
+Proof using.
+  intros G sc sc' EQ s s' EQS.
+  unfold iord_coherent. 
+  split; intros HH.
+  { now rewrite <- EQS, <- EQ. }
+  now rewrite EQS, EQ.
+Qed.
+
+Section IordCoherency.
+  Variables (tc: trav_label -> Prop) (G: execution) (sc: relation actid). 
+  Hypothesis (TCOH: tls_coherent G tc).
+  Hypotheses (WF: Wf G) (CONS: imm_consistent G sc).
+
+  Implicit Types
+           (ICOH: iord_coherent G sc tc)
+           (ICOHs: iord_simpl_coherent G sc tc).
+  
+
+  Notation "'sb'" := (sb G).
+  Notation "'rmw'" := (rmw G).
+  Notation "'data'" := (data G).
+  Notation "'addr'" := (addr G).
+  Notation "'ctrl'" := (ctrl G).
+  Notation "'rf'" := (rf G).
+  Notation "'co'" := (co G).
+  Notation "'coe'" := (coe G).
+  Notation "'fr'" := (fr G).
+
+  Notation "'fwbob'" := (fwbob G).
+  Notation "'ppo'" := (ppo G).
+  Notation "'ar'" := (ar G sc).
+  Notation "'fre'" := (fre G).
+  Notation "'rfi'" := (rfi G).
+  Notation "'rfe'" := (rfe G).
+  Notation "'deps'" := (deps G).
+  Notation "'detour'" := (detour G).
+
+  Notation "'lab'" := (lab G).
+  Notation "'loc'" := (loc lab).
+  Notation "'val'" := (val lab).
+  Notation "'mod'" := (Events.mod lab).
+  Notation "'same_loc'" := (same_loc lab).
+  
+  Notation "'E'" := (acts_set G).
+  Notation "'R'" := (fun x => is_true (is_r lab x)).
+  Notation "'W'" := (fun x => is_true (is_w lab x)).
+  Notation "'F'" := (fun x => is_true (is_f lab x)).
+  Notation "'Sc'" := (fun x => is_true (is_sc lab x)).
+  Notation "'RW'" := (R ∪₁ W).
+  Notation "'FR'" := (F ∪₁ R).
+  Notation "'FW'" := (F ∪₁ W).
+  Notation "'R_ex'" := (fun a => is_true (R_ex lab a)).
+  Notation "'W_ex'" := (W_ex G).
+  Notation "'W_ex_acq'" := (W_ex ∩₁ (fun a => is_true (is_xacq lab a))).
+  Notation "'Rel'" := (fun x => is_true (is_rel lab x)).
+
+  Lemma tlsc_w_covered_issued ICOH:
+    tlsC tc ∩₁ (event ↓₁ W) ⊆₁ event ↓₁ (event ↑₁ tlsI tc).
+  (* (fun ae => mkTL ta_issue (event ae)) ↓₁ (tlsC ∩₁ (event ↓₁ W)) ⊆₁ tlsI. *)
+  Proof using TCOH.
+    destruct TCOH. unfold tlsC, tlsI.
+    unfolder. ins. desc. destruct x as [a e]. ins. subst.
+    
+    exists (mkTL ta_issue e). splits; eauto.
+    destruct (tls_coh_exec _ H) as [Il | EXl].
+    { apply tls_coh_init. split; [basic_solver| ]. 
+      apply init_tls_EI in Il. auto. }
+    red in ICOH. apply ICOH.     
+    red. eexists. apply seq_eqv_r. split; eauto.
+    red. apply exec_tls_ENI in EXl. red. splits; try by vauto.
+    do 4 left. right. red. basic_solver 10. 
+  Qed.
+  
+  Let E_ENI := E × (E \₁ is_init).
+
+  Lemma sb_E_ENI: sb ⊆ E_ENI. 
+  Proof using. rewrite wf_sbE, no_sb_to_init. basic_solver. Qed. 
+
+  Lemma co_E_ENI (SCPL: sc_per_loc G): co ⊆ E_ENI. 
+  Proof using WF. rewrite wf_coE, no_co_to_init; auto. basic_solver. Qed. 
+
+  Lemma rf_E_ENI : rf ⊆ E_ENI. 
+  Proof using WF. rewrite wf_rfE, no_rf_to_init; auto. basic_solver. Qed. 
+
+  Lemma fr_E_ENI (SCPL: sc_per_loc G) : fr ⊆ E_ENI. 
+  Proof using WF. rewrite wf_frE, no_fr_to_init; auto. basic_solver. Qed. 
+
+  Lemma no_ar_to_init_alt:
+    ar ≡ ar ⨾ ⦗set_compl is_init⦘. 
+  Proof using CONS WF.
+    forward eapply no_ar_to_init; eauto. basic_solver 10.
+    Unshelve. all: eauto.
+  Qed. 
+
+  Lemma ar_E_ENI: ar ⊆ E_ENI. 
+  Proof using WF CONS.
+    rewrite wf_arE, no_ar_to_init_alt; auto; [| apply CONS]. basic_solver.
+  Qed.
+
+  Lemma sc_E_ENI (WFSC: wf_sc G sc): sc ⊆ E_ENI. 
+  Proof using WF.
+    rewrite wf_scE, (@no_sc_to_init _ WF _ WFSC); eauto. basic_solver.
+  Qed.
+
+  Lemma E_ENI_trans: transitive E_ENI.
+  Proof using. unfold E_ENI. basic_solver. Qed.
+
+  Lemma iord_simpl_E_ENI:
+    iord_simpl G sc ⊆ event ↓ E_ENI^?.
+  Proof using WF CONS. 
+    unfold iord_simpl. unfold SB, RF, FWBOB, AR, IPROP, PROP.
+    rewrite ppo_in_sb, fwbob_in_sb; auto. rewrite inclusion_inter_l1 with (r := sb).
+    rewrite ?sb_E_ENI, ?rf_E_ENI, ?co_E_ENI, ?fr_E_ENI, ?ar_E_ENI, ?sc_E_ENI; auto.
+    2: by apply CONS.
+    2: { apply imm_s_hb.coherence_sc_per_loc, CONS. } 
+    rewrite <- !seqA. 
+    repeat (rewrite ?(@rt_of_trans _ E_ENI), ?(@rewrite_trans _ E_ENI),
+             ?unionK, ?(@rewrite_trans _ E_ENI),
+             ?(@rewrite_trans_seq_cr_cr _ E_ENI), ?(@ct_of_trans _ E_ENI)
+           ); auto using E_ENI_trans.
+    repeat rewrite inclusion_seq_eqv_l, inclusion_seq_eqv_r. basic_solver 10.
+  Qed.
+
+  Lemma iord_simpl_tc_doma:
+    doma (iord_simpl G sc ⨾ ⦗tc⦘) (event ↓₁ E).
+  Proof using WF CONS TCOH.
+    rewrite iord_simpl_E_ENI; auto. rewrite crE, map_rel_union, seq_union_l.
+    apply union_doma.
+    { rewrite tlsc_E; eauto. unfolder. ins. desc. congruence. }
+    unfold E_ENI. basic_solver.
+  Qed. 
+
+  Lemma set_compl_set_mapC {A B: Type} (d: B -> Prop) (f: A -> B):
+    set_compl (f ↓₁ d) ≡₁  (f ↓₁ set_compl d).
+  Proof using. basic_solver. Qed. 
+
+  Lemma iord_coh_implies_iord_simpl_coh ICOH:
+    dom_rel (iord_simpl G sc ⨾ ⦗tc⦘) ⊆₁ tc. 
+  Proof using WF CONS TCOH.
+    rewrite set_split_complete with (s' := dom_rel _) (s := event ↓₁ is_init).
+    forward eapply iord_simpl_tc_doma as IS_DOM%doma_rewrite; eauto.
+
+    apply set_subset_union_l. split.
+    { rewrite IS_DOM.     
+      destruct TCOH. rewrite <- tls_coh_init at 2. unfold init_tls.
+      rewrite set_pair_alt, set_map_inter.
+      rewrite <- set_interA. apply set_subset_inter; [| reflexivity].  
+      rewrite dom_eqv1, set_interC. apply set_subset_inter; [| reflexivity].
+      unfold iord_simpl. unfold SB, RF, FWBOB, AR, IPROP, PROP.
+      basic_solver 10. }
+    
+    rewrite set_interC, <- dom_eqv1.
+    red in ICOH. rewrite <- ICOH at 2. apply dom_rel_mori.
+    unfold iord. fold iord_simpl.
+    rewrite restr_relE. rewrite !seqA, seq_eqvC. 
+    rewrite set_minusE, set_map_inter, id_inter.
+    rewrite !seqA, seq_eqvC.
+    rewrite <- seqA with (r3 := ⦗_⦘ ⨾ ⦗_⦘). rewrite <- seqA with (r2 := _ ⨾ ⦗tc⦘).
+    rewrite set_compl_set_mapC.
+    etransitivity.
+    2: { apply seq_mori; [reflexivity| ].
+         rewrite <- id_inter. apply domb_rewrite.
+         rewrite iord_simpl_E_ENI; auto.
+         rewrite crE, map_rel_union. repeat case_union _ _. apply union_domb.
+         { rewrite (@tlsc_E G tc) at 1; eauto.
+           unfolder. ins. desc. split; congruence. }
+         unfold E_ENI. basic_solver. }
+    apply doma_rewrite. rewrite IS_DOM. basic_solver.
+  Qed. 
+
+  Lemma iord_simpl_coh_implies_iord_coh ICOHs:
+    iord_coherent G sc tc. 
+  Proof using. 
+    red. erewrite dom_rel_mori; [by apply ICOHs| ].
+    unfold iord, iord_simpl. basic_solver 10.
+  Qed.
+
+  Lemma iord_coh_clos_refl ICOH:
+    dom_rel ((iord G sc)^? ⨾ ⦗tc⦘) ⊆₁ tc. 
+  Proof using.
+    rewrite crE, seq_union_l, seq_id_l, dom_union.
+    red in ICOH. rewrite ICOH. basic_solver.
+  Qed.
+
+  Lemma iord_simpl_coh_clos_refl ICOHs:
+    dom_rel ((iord_simpl G sc)^? ⨾ ⦗tc⦘) ⊆₁ tc. 
+  Proof using.
+    rewrite crE, seq_union_l, seq_id_l, dom_union.
+    red in ICOHs. rewrite ICOHs. basic_solver.
+  Qed.
+
+End IordCoherency.
+
